messageInvariantPrototypes/paxos/decentralizedMonotonic/distributedSystem.dfy
@@ -80,6 +80,13 @@ module DistributedSystem {
       && AcceptorHost.GroupWF(c.acceptorConstants, acceptors, c.f)
       && LearnerHost.GroupWF(c.learnerConstants, learners, c.f)
     }
+
+    ghost predicate LeaderCanPropose(c: Constants, ldr: LeaderId) 
+    requires WF(c)
+    requires c.ValidLeaderIdx(ldr)
+    {
+      leaders[ldr].CanPropose(c.leaderConstants[ldr])
+    }
   }
 
   ghost predicate Init(c: Constants, v: Variables)
